LeanColls/Classes/Map.lean
@@ -33,23 +33,23 @@ class Map (C : Type u) (κ : outParam (Type v)) (τ : outParam (Type w))
   extends MultiBag C (κ × τ) where
   /-- The [Bag] instance providing functions on this collection's [KeySet]. -/
   toBagKeySet : Bag.ReadOnly (Map.KeySet C) κ
-  /-- Look up `k` in collection `c` -/
-  get? : (c : C) → (k : κ) → Option τ
-  /-- Alter the entry at key `k` in `c`.
+  /-- Look up `k` in collection `cont` -/
+  get? : (cont : C) → (k : κ) → Option τ
+  /-- Alter the entry at key `k` in `cont`.
     The `f` is given the current value at `k`,
     or none if not defined at `k`.
     If `f` returns `none`, `k` is erased. -/
-  alter : (c : C) → (k : κ) → (f : Option τ → Option τ) → C
-  /-- Set the entry at key `k` to `v` in `c`. -/
-  set : (c : C) → (k : κ) → (v : τ) → C := (alter · · <| Function.const _ <| some ·)
+  alter : (cont : C) → (k : κ) → (f : Option τ → Option τ) → C
+  /-- Set the entry at key `k` to `v` in `cont`. -/
+  set : (cont : C) → (k : κ) → (v : τ) → C := (alter · · <| Function.const _ <| some ·)
   /-- Modify the value at key `k`, if present, by applying `f`.
     Otherwise leave the map unchanged. -/
-  modify : (c : C) → (k : κ) → (f : τ → τ) → C := (alter · · <| Option.map · )
+  modify : (cont : C) → (k : κ) → (f : τ → τ) → C := (alter · · <| Option.map · )
   /-- Remove the entry at key `k`, if present. -/
-  remove : (c : C) → (k : κ) → C := (alter · · (Function.const _ none))
+  remove : (cont : C) → (k : κ) → C := (alter · · (Function.const _ none))
 
 attribute [instance] Map.toBagKeySet
 
 namespace Map
 
-def keySet (c : C) : KeySet C := ⟨c⟩
+def keySet (cont : C) : KeySet C := ⟨cont⟩
