CONVENTIONS.md
@@ -1,0 +1,4 @@
+## Naming Conventions
+
+- Container types: `C` (with subscripts, if multiple)
+- Container arguments: `cont : C`
